\documentclass[10pt,letterpaper]{article}
\usepackage{mymacros}

\title{Cosmological Perturbation Theory Notes}
\author{}
\date{}

\begin{document}
\section*{Harmonic Flat Space Conformal Transformation}
Harmonic condition:
\[
	\pd_\mu h^\mu{}_\nu - \frac12 \pd_\nu h^\mu{}_\mu=0
\]
\[
	\del_\mu h^\mu{}_\nu - \frac12 \del_\nu h^\mu{}_\mu=0.
\]
Conformal transformation:
\[
	\Omega^2 g_{\mu\nu} = \bar g_{\mu\nu}
\]
\[
	 \Omega^{-2} g^{\mu\nu}=\bar g^{\mu\nu} 
\]
\[
	h^\mu{}_\nu = g^{(0)}_{\rho\nu} h^{\mu\rho} = (\Omega^{-2} \bar g^{(0)}_{\rho\nu}) (\Omega^2 \bar h^{\mu\rho} ) = \bar h^\mu{}_\nu
\]
The following will be useful within our gauge transformation:
\[
	\Gamma^{\lambda}_{\mu\nu} = \bar\Gamma^{\lambda}_{\mu\nu} -  \Omega^{-1}\plr{ \delta^\lambda_\nu \pd_\mu \Omega + \delta^\lambda_\mu \pd_\nu \Omega - n_{\mu\nu}n^{\lambda\rho}\pd_\rho \Omega}
\]
\ba
	\del_\mu h^\mu{}_\nu - \frac12 \del_\nu h^\mu{}_\mu&= \pd_\mu h^\mu{}_\nu + \Gamma^\mu_{\mu\rho} h^\rho{}_\nu - \Gamma^\rho_{\mu\nu} h^\mu{}_\rho
	-\frac12\pd_\nu h^\mu{}_\mu\\
	&= \pd_\mu \bar h^\mu{}_\nu + \bar \Gamma^\mu_{\mu\rho}\bar  h^\rho{}_\nu - \bar \Gamma^\rho_{\mu\nu} h^\mu{}_\rho
	-\frac12\pd_\nu \bar h^\mu{}_\mu-4\Omega^{-1}\bar h^\rho{}_\nu \pd_\rho\Omega 
	+\Omega^{-1}\bar h^{\mu}{}_\rho \plr{ \delta^\rho_\nu \pd_\mu\Omega + \delta^\rho_\mu \pd_\nu\Omega - \eta^{\rho\alpha}\eta_{\mu\nu}\pd_\alpha\Omega} \\
	&= \bar\del_\mu\bar h^{\mu}{}_\nu - \frac12 \bar \del_\nu \bar h^\mu{}_\mu-4\Omega^{-1}\bar h^\rho{}_\nu \pd_\rho\Omega 
	+\Omega^{-1}\bar h^{\mu}{}_\rho \plr{ \delta^\rho_\nu \pd_\mu\Omega + \delta^\rho_\mu \pd_\nu\Omega - \eta^{\rho\alpha}\eta_{\mu\nu}\pd_\alpha\Omega}\\
	&=\bar \del_\mu \bar h^\mu{}_\nu - \frac12 \bar \del_\nu \bar h^\mu{}_\mu - 4\Omega^{-1} \bar h^\rho{}_\nu  \pd_\rho \Omega + \Omega^{-1} \bar h^\mu{}_\mu \pd_\nu \Omega
\ea
In a conformal to flat space, we need to work in the gauge 
\[
	 \bar \del_\mu \bar h^\mu{}_\nu - \frac12 \bar \del_\nu \bar h^\mu{}_\mu = 4\Omega^{-1} \bar h^\rho{}_\nu  \pd_\rho \Omega - \Omega^{-1} h^\mu{}_\mu \pd_\nu \Omega
\]
%Einstein Perturbation:
%\[
%	G_{\mu\nu} = R_{\mu\nu} - \frac12 g_{\mu\nu}R
%\]
%\[
%	\delta G_{\mu\nu} = \delta R_{\mu\nu} - \frac12 h_{\mu\nu}R - \frac12 g_{\mu\nu}\plr{
%	h_{\alpha\beta}R^{\alpha\beta} + g^{\alpha\beta}\delta R_{\alpha\beta}}
%\]
Perturbation of Ricci Tensor:
\[
	R_{\mu\nu} = T_{\mu\nu} -\frac12g_{\mu\nu}T^\lambda{}_\lambda \equiv S_{\mu\nu}
\]
\[
	\delta R_{\mu\nu} = \delta S_{\mu\nu}
\]
Weinberg (10.9.3)
\ba
	\delta R_{\mu\nu} &= (\delta \Gamma^{\lambda}_{\mu\lambda})_{;\nu} - (\delta \Gamma^{\lambda}_{\mu\nu})_{;\lambda}\\
	&= \frac12 g^{\lambda\rho}\blr{ (h_{\lambda\rho})_{;\mu;\nu} - (h_{\rho\mu})_{;\nu;\lambda} - (h_{\rho\nu})_{;\mu;\lambda}
	+(h_{\mu\nu})_{;\rho;\lambda}}\\
	&= \frac12 \plr{ \del_\nu \del_\mu h^\lambda{}_\lambda - \del_\lambda \del_\nu h^\lambda{}_\mu  - \del_\lambda \del_\mu h^\lambda{}_\nu + \del_\lambda \del ^\lambda h_{\mu\nu}}
\ea
%\ba
%	\delta G_{\mu\nu} &=  \frac12 \plr{ \del_\nu \del_\mu h^\lambda{}_\lambda - \del_\lambda \del_\nu h^\lambda{}_\mu  - \del_\lambda \del_\mu h^\lambda{}_\nu + \del_\lambda \del ^\lambda h_{\mu\nu}} - \frac12 h_{\mu\nu}R - \frac12 g_{\mu\nu}h_{\alpha\beta}R^{\alpha\beta}\\  
%	&\quad -\frac14 g_{\mu\nu} g^{\alpha\beta}  \plr{ \del_\beta \del_\alpha h^\lambda{}_\lambda - \del_\lambda \del_\beta h^\lambda{}_\alpha  - \del_\lambda \del_\alpha h^\lambda{}_\beta + \del_\lambda \del ^\lambda h_{\alpha\beta}}\\
%	&=  \frac12 \plr{ \del_\nu \del_\mu h^\lambda{}_\lambda - \del_\lambda \del_\nu h^\lambda{}_\mu  - \del_\lambda \del_\mu h^\lambda{}_\nu + \del_\lambda \del ^\lambda h_{\mu\nu}} - \frac12 h_{\mu\nu}R - \frac12 g_{\mu\nu}h_{\alpha\beta}R^{\alpha\beta}\\  
%	&\quad -\frac14 g_{\mu\nu}  \plr{ 2\del_\beta \del^\beta h^\lambda{}_\lambda -2 \del^\alpha\del_\lambda h^\lambda{}_\alpha }\\
%		&=  \frac12 \plr{ \del_\nu \del_\mu h^\lambda{}_\lambda - \del_\lambda \del_\nu h^\lambda{}_\mu  - \del_\lambda \del_\mu h^\lambda{}_\nu + \del_\lambda \del ^\lambda h_{\mu\nu}} - \frac12 h_{\mu\nu}R - \frac12 g_{\mu\nu}h_{\alpha\beta}R^{\alpha\beta}\\  
%	&\quad -\frac12 g_{\mu\nu}  \plr{ \del_\beta \del^\beta h^\lambda{}_\lambda - \del^\alpha\del_\lambda h^\lambda{}_\alpha }\\
%\ea
%\[
%	G_{\mu\nu} = R_{\mu\nu} - \frac12 g_{\mu\nu}R=T_{\mu\nu}
%\]
%\[
%	G^\mu{}_\mu = R-2R = -R = T^\mu{}_\mu
%\]

\[
	\delta R_{\mu\nu} = \frac12 \plr{ \del_\nu \del_\mu h^\lambda{}_\lambda - \del_\lambda \del_\nu h^\lambda{}_\mu  - \del_\lambda \del_\mu h^\lambda{}_\nu + \del_\lambda \del ^\lambda h_{\mu\nu}}
\]
\[
	 \bar \del_\mu \bar h^\mu{}_\nu - \frac12 \bar \del_\nu \bar h^\mu{}_\mu = 4\Omega^{-1} \bar h^\rho{}_\nu  \pd_\rho \Omega - \Omega^{-1} h^\mu{}_\mu \pd_\nu \Omega
\]
Referring to Mannheim (35), we may use the covariant interchange identity to express the Ricci variation as
\[
	\delta R_{\mu\nu} = \frac12\plr{ \del_\nu \del_\mu h^\lambda{}_\lambda - \del_\nu \del_\lambda h^\lambda{}_\mu - \del_\mu \del_\lambda h^\lambda{}_\nu + \del_\lambda \del^\lambda h_{\mu\nu}}
	+\frac12 g^{\lambda\rho}\plr{ h^\sigma{}_\rho R_{\sigma \nu \mu \lambda}+h^\sigma{}_\rho R_{\sigma \mu \nu \lambda} - h^{\sigma}{}_\mu R_{\rho\sigma \nu \lambda} - h^\sigma{}_\nu R_{\rho\sigma\mu\lambda}}.
\]
Substituting our gauge choice for the middle two covariant derivative terms
\ba
	\delta R_{\mu\nu} &= \frac12\plr{ \del_\nu \del_\mu h^\lambda{}_\lambda - \del_\nu \del_\lambda h^\lambda{}_\mu - \del_\mu \del_\lambda h^\lambda{}_\nu + \del_\lambda \del^\lambda h_{\mu\nu}}
	+\frac12 g^{\lambda\rho}\plr{ h^\sigma{}_\rho R_{\sigma \nu \mu \lambda}+h^\sigma{}_\rho R_{\sigma \mu \nu \lambda} - h^{\sigma}{}_\mu R_{\rho\sigma \nu \lambda} - h^\sigma{}_\nu R_{\rho\sigma\mu\lambda}}\\
	&=  \frac12\plr{ \del_\nu \del_\mu h^\lambda{}_\lambda - \frac12 \del_\nu \del_\mu h^\lambda{}_\lambda - \frac12 \del_\mu \del_\nu h^\lambda{}_\lambda + \del_\lambda \del^\lambda h_{\mu\nu}}
	+\frac12 g^{\lambda\rho}\plr{ h^\sigma{}_\rho R_{\sigma \nu \mu \lambda}+h^\sigma{}_\rho R_{\sigma \mu \nu \lambda} - h^{\sigma}{}_\mu R_{\rho\sigma \nu \lambda} - h^\sigma{}_\nu R_{\rho\sigma\mu\lambda}}\\
	&\quad- \del_\nu \plr{ 4\Omega^{-1} \bar h^\rho{}_\mu  \pd_\rho \Omega - \Omega^{-1} h^\lambda{}_\lambda \pd_\mu \Omega} -\del_\mu \plr{4\Omega^{-1} \bar h^\rho{}_\nu  \pd_\rho \Omega - \Omega^{-1} h^\lambda{}_\lambda \pd_\nu \Omega}\\
	&= \frac12 \del_\lambda \del^\lambda h_{\mu\nu}+\frac12 g^{\lambda\rho}\plr{ h^\sigma{}_\rho R_{\sigma \nu \mu \lambda}+h^\sigma{}_\rho R_{\sigma \mu \nu \lambda} - h^{\sigma}{}_\mu R_{\rho\sigma \nu \lambda} - h^\sigma{}_\nu R_{\rho\sigma\mu\lambda}}\\
	&\quad- \frac12\del_\nu \plr{ 4\Omega^{-1} \bar h^\rho{}_\mu  \pd_\rho \Omega - \Omega^{-1} h^\lambda{}_\lambda \pd_\mu \Omega} -\frac12\del_\mu \plr{4\Omega^{-1} \bar h^\rho{}_\nu  \pd_\rho \Omega - \Omega^{-1} h^\lambda{}_\lambda \pd_\nu \Omega}\\
\ea
From here we would like to evaluate the Riemann tensor for a conformal to flat metric. From Weinberg (6.1.5) we have
%\ba
%	R_{\lambda\mu\nu \kappa} = \frac12 \plr{ \pd_\kappa\pd_\mu g_{\lambda\nu} - \pd_\kappa\pd_\lambda g_{\mu\nu} - \pd_\mu\pd_\nu g_{\lambda\kappa} + \pd_\nu\pd_\lambda
%	g_{\mu\kappa}}+ g_{\rho\sigma}\plr{ \Gamma^\rho_{\nu\lambda}\Gamma^\sigma_{\mu\kappa} - \Gamma^\rho_{\kappa\lambda}\Gamma^\sigma_{\mu\nu}}.
%\ea
%\[
%	\Omega^2 g_{\mu\nu} = \bar g_{\mu\nu}
%\]
%\[
%	 \Omega^{-2} g^{\mu\nu}=\bar g^{\mu\nu} 
%\]
%We will need an expression for the Christoffel symbol:
%\ba
%	\Gamma^\lambda_{\mu\nu} &= \frac{g^{\lambda\rho}}{2} \plr{ \pd_\mu g_{\rho\nu} + \pd_\nu g_{\rho \mu}-\pd_\rho g_{\mu\nu}}\\
%	&= n^{\lambda\rho}\Omega^{-1}\plr{ \eta_{\rho\nu}\pd_\mu \Omega + \eta_{\rho\mu} \pd_\nu \Omega - \eta_{\mu\nu}\pd_\rho \Omega}\\
%	&= \Omega^{-1}\plr{ \delta^\lambda_\nu \pd_\mu \Omega + \delta^\lambda_\mu \pd_\nu \Omega - n_{\mu\nu}n^{\lambda\rho}\pd_\rho \Omega}
%\ea
%\ba
%	\Gamma^\rho_{\nu\lambda}\Gamma^\sigma_{\mu\kappa} - \Gamma^\rho_{\kappa\lambda}\Gamma^\sigma_{\mu\nu}&= 
%	\Omega^{-2} \plr{ \delta^\rho_\nu \pd_\lambda \Omega + \delta^\rho_\lambda \pd_\nu \Omega - n_{\nu\lambda}n^{\rho\sigma}\pd_\sigma \Omega}
%	\plr{\delta^\sigma_\mu \pd_\kappa \Omega + \delta^\sigma_\kappa \pd_\mu\Omega - n_{\mu\kappa}n^{\sigma\alpha}\pd_\alpha \Omega}\\
%	&\quad - \Omega^{-2} \plr{ \delta^\rho_\kappa \pd_\lambda \Omega + \delta^\rho_\lambda \pd_\kappa \Omega - n_{\kappa\lambda}n^{\rho\alpha}\pd_\alpha \Omega}
%	\plr{ \delta^\sigma_\mu \pd_\nu \Omega + \delta^\sigma_\nu \pd_\mu\Omega - \eta_{\mu\nu}\eta^{\sigma\beta}\pd_\beta \Omega}
%\ea
%\ba
%		\Omega^2\Gamma^\rho_{\nu\lambda}\Gamma^\sigma_{\mu\kappa} &=\plr{ \delta^\rho_\nu \pd_\lambda \Omega + \delta^\rho_\lambda \pd_\nu \Omega - n_{\nu\lambda}n^{\rho\sigma}\pd_\sigma \Omega}
%	\plr{\delta^\sigma_\mu \pd_\kappa \Omega + \delta^\sigma_\kappa \pd_\mu\Omega - n_{\mu\kappa}n^{\sigma\alpha}\pd_\alpha \Omega}\\
%		&=\plr{ \delta^\rho_\nu \delta^\sigma_\mu \pd_\lambda\Omega \pd_\kappa\Omega + \delta^\rho_\nu \delta^\sigma_\kappa\pd_\lambda\Omega \pd_\mu\Omega
%		-\delta^\rho_\nu \eta_{\mu\kappa}\eta^{\sigma\alpha}\pd_\lambda \Omega \pd_\alpha \Omega}\\
%		&\quad + \plr{\delta^\rho_\lambda \delta^\sigma_\mu \pd_\nu\Omega \pd_\kappa\Omega + \delta^\rho_\lambda \delta^\sigma_\kappa \pd_\nu \Omega \pd_ \mu \Omega
%		-\delta^\rho_\lambda \eta_{\mu\kappa}\eta^{\sigma\alpha}\pd_\nu\Omega \pd_\alpha\Omega}\\
%		&\quad-\eta_{\mu\kappa}\eta^{\sigma\alpha}\pd_\alpha\Omega \plr{ \delta^\rho_\nu \pd_\lambda \Omega + \delta^\rho_\lambda \pd_\nu \Omega - n_{\nu\lambda}n^{\rho\sigma}\pd_\sigma \Omega}
%\ea
%\ba
%		\Omega^2\Gamma^\rho_{\kappa\lambda}\Gamma^\sigma_{\mu\nu} &=\plr{ \delta^\rho_\kappa \pd_\lambda \Omega + \delta^\rho_\lambda \pd_\kappa \Omega - n_{\kappa\lambda}n^{\rho\alpha}\pd_\alpha \Omega}
%	\plr{ \delta^\sigma_\mu \pd_\nu \Omega + \delta^\sigma_\nu \pd_\mu\Omega - \eta_{\mu\nu}\eta^{\sigma\beta}\pd_\beta \Omega}\\
%		&=\plr{ \delta^\rho_\kappa\delta^\sigma_\mu \pd_\lambda \Omega \pd_\nu \Omega + \delta^\rho_\kappa\delta^\sigma_\nu \pd_\lambda\Omega \pd_\mu\Omega - \delta^\rho_\kappa\eta_{\mu\nu}\eta^{\sigma\beta}\pd_\lambda \Omega \pd_\beta \Omega} \\
%		&\quad + \plr{ \delta^\rho_\lambda \delta^\sigma_\mu \pd_\kappa \Omega \pd_\nu \Omega +\delta^\rho_\lambda \delta^\sigma_\nu \pd_\kappa\Omega \pd_\mu \Omega
%		-\delta^\rho_\kappa \eta_{\mu\nu}\eta^{\sigma\beta}\pd_\lambda\Omega \pd_\beta\Omega}\\
%		&\quad -\eta_{\mu\nu}\eta^{\sigma\beta}\pd_\beta\Omega\plr{ \delta^\rho_\kappa \pd_\lambda \Omega + \delta^\rho_\lambda \pd_\kappa \Omega - n_{\kappa\lambda}n^{\rho\alpha}\pd_\alpha \Omega}
%\ea
%\ba
%	g_{\rho\sigma}\Gamma^\rho_{\nu\lambda}\Gamma^\sigma_{\mu\kappa} &= g_{\rho\sigma}[
%	\plr{ \delta^\rho_\nu \delta^\sigma_\mu \pd_\lambda\Omega \pd_\kappa\Omega + \delta^\rho_\nu \delta^\sigma_\kappa\pd_\lambda\Omega \pd_\mu\Omega
%		-\delta^\rho_\nu \eta_{\mu\kappa}\eta^{\sigma\alpha}\pd_\lambda \Omega \pd_\alpha \Omega}\\
%		&\quad + \plr{\delta^\rho_\lambda \delta^\sigma_\mu \pd_\nu\Omega \pd_\kappa\Omega + \delta^\rho_\lambda \delta^\sigma_\kappa \pd_\nu \Omega \pd_ \mu \Omega
%		-\delta^\rho_\lambda \eta_{\mu\kappa}\eta^{\sigma\alpha}\pd_\nu\Omega \pd_\alpha\Omega}\\
%		&\quad-\eta_{\mu\kappa}\eta^{\sigma\alpha}\pd_\alpha\Omega \plr{ \delta^\rho_\nu \pd_\lambda \Omega + \delta^\rho_\lambda \pd_\nu \Omega - n_{\nu\lambda}n^{\rho\sigma}\pd_\sigma \Omega}]\\
%		&= \eta_{\mu\nu} \pd_\lambda\Omega\pd_\kappa\Omega + \eta_{\nu\kappa}\pd_\lambda\Omega\pd_\mu\Omega - \eta_{\mu\kappa}\pd_\lambda\Omega\pd_\nu\Omega\\
%		&\quad+ \eta_{\lambda\mu}\pd_\nu\Omega \pd_\kappa \Omega + \eta_{\lambda\kappa}\pd_\nu\Omega \pd_\mu\Omega - \eta_{\mu\kappa}\pd_\nu\Omega\pd_\lambda\Omega
%		\\ &\quad -2 \eta_{\mu\kappa} \pd_\nu\Omega\pd_\lambda\Omega+4\eta_{\mu\kappa}\eta_{\nu\lambda}\pd_\sigma\Omega \pd^\sigma\Omega\\
%		&= \eta_{\mu\nu} \pd_\lambda\Omega\pd_\kappa\Omega + \eta_{\nu\kappa}\pd_\lambda\Omega\pd_\mu\Omega+ \eta_{\lambda\mu}\pd_\nu\Omega \pd_\kappa \Omega + \eta_{\lambda\kappa}\pd_\nu\Omega \pd_\mu\Omega
%		\\ &\quad -4 \eta_{\mu\kappa} \pd_\nu\Omega\pd_\lambda\Omega+4\eta_{\mu\kappa}\eta_{\nu\lambda}\pd_\sigma\Omega \pd^\sigma\Omega
%\ea
%\ba
%	g_{\rho\sigma}\Gamma^\rho_{\kappa\lambda}\Gamma^\sigma_{\mu\nu}&= g_{\rho\sigma} [\plr{ \delta^\rho_\kappa\delta^\sigma_\mu \pd_\lambda \Omega \pd_\nu \Omega + \delta^\rho_\kappa\delta^\sigma_\nu \pd_\lambda\Omega \pd_\mu\Omega - \delta^\rho_\kappa\eta_{\mu\nu}\eta^{\sigma\beta}\pd_\lambda \Omega \pd_\beta \Omega} \\
%		&\quad + \plr{ \delta^\rho_\lambda \delta^\sigma_\mu \pd_\kappa \Omega \pd_\nu \Omega +\delta^\rho_\lambda \delta^\sigma_\nu \pd_\kappa\Omega \pd_\mu \Omega
%		-\delta^\rho_\kappa \eta_{\mu\nu}\eta^{\sigma\beta}\pd_\lambda\Omega \pd_\beta\Omega}\\
%		&\quad -\eta_{\mu\nu}\eta^{\sigma\beta}\pd_\beta\Omega\plr{ \delta^\rho_\kappa \pd_\lambda \Omega + \delta^\rho_\lambda \pd_\kappa \Omega - n_{\kappa\lambda}n^{\rho\alpha}\pd_\alpha \Omega}]\\
%		&= \eta_{\mu\kappa}\pd_\lambda\Omega \pd_\nu\Omega + \eta_{\kappa\nu}\pd_\lambda\Omega \pd_\mu\Omega - \eta_{\mu\nu} \pd_{\lambda}\Omega\pd_\kappa \Omega\\
%		&\quad + \eta_{\lambda\mu}\pd_\kappa\Omega\pd_\nu\Omega + \eta_{\lambda\nu}\pd_\kappa\Omega \pd_\mu\Omega - \eta_{\mu\nu}\pd_\lambda\Omega\pd_\kappa\Omega\\
%		&\quad - 2\eta_{\mu\nu}\pd_\lambda\Omega\pd_\kappa\Omega +4\eta_{\mu\nu}\eta_{\lambda\kappa}\pd_\sigma \Omega \pd^\sigma \Omega\\
%		&=  \eta_{\mu\kappa}\pd_\lambda\Omega \pd_\nu\Omega + \eta_{\kappa\nu}\pd_\lambda\Omega \pd_\mu\Omega+ \eta_{\lambda\mu}\pd_\kappa\Omega\pd_\nu\Omega + \eta_{\lambda\nu}\pd_\kappa\Omega \pd_\mu\Omega \\
%		&\quad - 4\eta_{\mu\nu}\pd_\lambda\Omega\pd_\kappa\Omega +4\eta_{\mu\nu}\eta_{\lambda\kappa}\pd_\sigma \Omega \pd^\sigma \Omega\\
%\ea
%\[
% 	g_{\rho\sigma}(\Gamma^\rho_{\nu\lambda}\Gamma^\sigma_{\mu\kappa}-\Gamma^\rho_{\kappa\lambda}\Gamma^\sigma_{\mu\nu})
% 	= 5\eta_{\mu\nu}\pd_\lambda\Omega\pd_\kappa\Omega -5\eta_{\mu\kappa}\pd_\nu\Omega\pd_\lambda\Omega+\eta_{\lambda\kappa}\pd_\nu\Omega\pd_\mu\Omega + \eta_{\lambda\nu}\pd_\kappa\Omega\pd_\mu\Omega + 4\eta_{\mu\kappa}\eta_{\nu\lambda}\pd_\sigma\Omega\pd^\sigma\Omega
% 	-4\eta_{\mu\nu}\eta_{\lambda\kappa}\pd_\sigma\Omega\pd^\sigma\Omega
%\]
%\vspace{100mm}
\[
	\Omega^2 g_{\mu\nu} = \bar g_{\mu\nu}
\]
\[
	 \Omega^{-2} g^{\mu\nu}=\bar g^{\mu\nu} 
\]

\[
	R^\lambda{}_{\mu\nu\kappa} = \pd_\kappa \Gamma^\lambda_{\mu\nu} - \pd_\nu \Gamma^\lambda_{\mu\kappa} + \Gamma^\eta_{\mu\nu}\Gamma^\lambda_{\kappa\eta}
	-\Gamma^\eta_{\mu\kappa}\Gamma^\lambda_{\nu\eta}.
\]
We will need an expression for the Christoffel symbol:
\ba
	\Gamma^\lambda_{\mu\nu} 
	&= \Omega^{-1}\plr{ \delta^\lambda_\nu \pd_\mu \Omega + \delta^\lambda_\mu \pd_\nu \Omega - n_{\mu\nu}n^{\lambda\rho}\pd_\rho \Omega}.
\ea
Now form the Riemann tensor
\ba
		R_{\lambda\mu\nu\kappa} &= g_{\lambda\rho}(\pd_\kappa \Gamma^\rho_{\mu\nu} - \pd_\nu \Gamma^\rho_{\mu\kappa} + \Gamma^\eta_{\mu\nu}\Gamma^\rho_{\kappa\eta}
	-\Gamma^\eta_{\mu\kappa}\Gamma^\rho_{\nu\eta})\\
	&= \Omega\plr{ \eta_{\lambda\nu} \pd_\mu \pd_\kappa \Omega + \eta_{\kappa\mu}\pd_\nu\pd_\lambda \Omega - \eta_{\mu\nu}\pd_\lambda\pd_\kappa \Omega -\eta_{\kappa\lambda}\pd_\mu\pd_\nu \Omega}+\eta_{\mu\kappa}\eta_{\lambda\nu}\pd_\alpha \Omega \pd^\alpha \Omega - \eta_{\kappa\lambda}\eta_{\mu\nu}\pd_\alpha \Omega\pd^\alpha\Omega\\
	&\quad
	+2\eta_{\mu\nu} \pd_\kappa \Omega\pd_\lambda\Omega - 2\eta_{\lambda\nu}\pd_\kappa \Omega \pd_\mu\Omega - 2\eta_{\kappa\mu}\pd_\lambda \Omega
	\pd_\nu\Omega + 2\eta_{\kappa\lambda}\pd_\mu \Omega \pd_\nu\Omega
\ea

\ba
	\delta R_{\mu\nu}&= \frac12 \del_\lambda \del^\lambda h_{\mu\nu}+\frac12 g^{\lambda\rho}\plr{ h^\sigma{}_\rho R_{\sigma \nu \mu \lambda}+h^\sigma{}_\rho R_{\sigma \mu \nu \lambda} - h^{\sigma}{}_\mu R_{\rho\sigma \nu \lambda} - h^\sigma{}_\nu R_{\rho\sigma\mu\lambda}}\\
	&\quad- \del_\nu \plr{ 4\Omega^{-1} \bar h^\rho{}_\mu  \pd_\rho \Omega - \Omega^{-1} h^\lambda{}_\lambda \pd_\mu \Omega} -\del_\mu \plr{4\Omega^{-1} \bar h^\rho{}_\nu  \pd_\rho \Omega - \Omega^{-1} h^\lambda{}_\lambda \pd_\nu \Omega}\\
\ea
\ba
	 \del_\nu \plr{ 4\Omega^{-1} \bar h^\rho{}_\mu  \pd_\rho \Omega - \Omega^{-1} h^\lambda{}_\lambda \pd_\mu \Omega}&=
	 4\Omega^{-1}\plr{ \del_\nu \bar h^\rho{}_\mu \pd_\rho \Omega + \bar h^\rho{}_\mu \del_\nu \del_\rho \Omega - \Omega^{-1}\bar h^{\rho}{}_\mu \pd_\nu \Omega \pd_\rho \Omega
	 }\\
	 &\quad -\Omega^{-1}\plr{ \pd_\nu \bar h^\lambda{}_\lambda \pd_\mu \Omega +\bar h^\lambda{}_\lambda \del_\nu \del_\mu \Omega -
	 \Omega^{-1} \bar h^\lambda{}_\lambda \pd_\nu \Omega \pd_\mu\Omega}\\
	 &=	 4\Omega^{-3}\eta^{\rho\kappa}\plr{ \del_\nu \bar h_{\kappa\mu} \pd_\rho \Omega + \bar h_{\kappa\mu} \del_\nu \del_\rho \Omega - \Omega^{-1}\bar h_{\kappa\mu} \pd_\nu \Omega \pd_\rho \Omega
	 }\\
	 &\quad -\Omega^{-3}\eta^{\lambda\kappa}\plr{ \pd_\nu \bar h_{\kappa\lambda} \pd_\mu \Omega +\bar h_{\kappa\lambda} \del_\nu \del_\mu \Omega -
	 \Omega^{-1} \bar h_{\kappa\lambda} \pd_\nu \Omega \pd_\mu\Omega}\\ \\
	 &=\Omega^{-3}\plr{ 4\eta^{\rho\kappa}\del_\nu h_{\kappa\mu}\pd_\rho\Omega +4\eta^{\rho\kappa}h_{\kappa\mu}\del_\nu\del_\rho \Omega -\eta^{\lambda\kappa}\pd_\nu h_{\kappa\lambda}
	 \pd_\mu\Omega - \eta^{\lambda\kappa}h_{\kappa\lambda}\del_\nu\del_\mu \Omega}\\
	 &\quad \Omega^{-4}\plr{ -4\eta^{\rho\kappa} h_{\kappa\mu}\pd_\nu\Omega \pd_\rho\Omega+\eta^{\lambda\kappa}h_{\kappa\lambda}\pd_\nu\Omega\pd_\mu\Omega}
\ea
\\
\[
	\del_\nu h_{\kappa\mu} = \pd_\nu h_{\kappa\mu} +\Omega^{-1}\plr{
	\eta^{\alpha\beta} \eta_{\mu\nu} h_{\kappa\alpha}\pd_\beta \Omega + \eta^{\alpha\beta}\eta_{\kappa\nu}h_{\mu\alpha}\pd_\beta\Omega - h_{\mu\nu}\pd_\kappa \Omega
	-h_{\kappa\nu}\pd_\mu\Omega - 2h_{\kappa\mu}\pd_\nu \Omega}
\]
\[
	\del_\nu\del_\rho \Omega = \pd_\rho\pd_\nu \Omega + \Omega^{-1}(\eta^{\alpha\beta}\eta_{\nu\rho}\pd_\alpha\Omega\pd_\beta \Omega - 2\pd_\nu \Omega \pd_\rho\Omega )
\]
\ba
	 \del_\nu \plr{ 4\Omega^{-1} \bar h^\rho{}_\mu  \pd_\rho \Omega - \Omega^{-1}\bar h^\lambda{}_\lambda \pd_\mu \Omega}&=\\
	 &\quad\Omega^{-3}\plr{  4\eta^{\rho\kappa} \pd_\nu h_{\kappa\mu}\pd_\rho\Omega +4\eta^{\rho\kappa}h_{\kappa\mu} \pd_\nu\pd_\rho\Omega - \eta^{\lambda\kappa}\pd_\nu
	 h_{\kappa\lambda}\pd_\mu\Omega - \eta^{\lambda\kappa}h_{\kappa\lambda}\pd_\nu\pd_\mu\Omega}\\
		 &+\Omega^{-4}(-4\eta^{\rho\kappa}h_{\kappa\mu}\pd_\nu\Omega \pd_\rho\Omega + \eta^{\lambda\kappa}h_{\kappa\lambda}\pd_\nu\Omega\pd_\mu\Omega
		 +4\eta^{\rho\kappa}\eta^{\alpha\beta}\eta_{\mu\nu}h_{\kappa\alpha}\pd_\beta\Omega\pd_\rho\Omega\\
		 &\qquad +4\eta^{\rho\kappa}\eta^{\alpha\beta}\eta_{\kappa\nu}h_{\mu\alpha}\pd_\beta\Omega\pd_\rho\Omega
		 -4\eta^{\rho\kappa}h_{\mu\nu}\pd_\kappa\Omega\pd_\rho\Omega-4\eta^{\rho\kappa}h_{\kappa\nu}\pd_\mu\Omega \pd_\rho\Omega\\
		 &\qquad -8\eta^{\rho\kappa}h_{\kappa\mu}\pd_\nu\Omega\pd_\rho\Omega+4\eta^{\rho\kappa}\eta^{\alpha\beta}\eta_{\nu\rho}h_{\kappa\mu}\pd_\alpha\Omega
		 \pd_\beta\Omega-8\eta^{\rho\kappa}h_{\kappa\mu}\pd_\nu\Omega\pd_\rho\Omega\\
		 &\qquad -\eta^{\lambda\kappa}\eta^{\alpha\beta}\eta_{\mu\nu}h_{\kappa\lambda}\pd_\alpha\Omega\pd_\beta\Omega
		 +2\eta^{\lambda\kappa}h_{\kappa\lambda}\pd_\nu\Omega\pd_\mu\Omega)\\ \\
		 &= \quad\Omega^{-3}\plr{  4\eta^{\rho\kappa} \pd_\nu h_{\kappa\mu}\pd_\rho\Omega +4\eta^{\rho\kappa}h_{\kappa\mu} \pd_\nu\pd_\rho\Omega - \eta^{\lambda\kappa}\pd_\nu
	 h_{\kappa\lambda}\pd_\mu\Omega - \eta^{\lambda\kappa}h_{\kappa\lambda}\pd_\nu\pd_\mu\Omega}\\
		 &\quad+\Omega^{-4}(3 \eta^{\lambda\kappa}h_{\kappa\lambda}\pd_\nu\Omega\pd_\mu\Omega
		 +4\eta^{\rho\kappa}\eta^{\alpha\beta}\eta_{\mu\nu}h_{\kappa\alpha}\pd_\beta\Omega\pd_\rho\Omega-4\eta^{\rho\kappa}h_{\kappa\nu}\pd_\mu\Omega \pd_\rho\Omega\\
		 &\qquad -16\eta^{\rho\kappa}h_{\kappa\mu}\pd_\nu\Omega\pd_\rho\Omega  -\eta^{\lambda\kappa}\eta^{\alpha\beta}\eta_{\mu\nu}h_{\kappa\lambda}\pd_\alpha\Omega\pd_\beta\Omega)\\
\ea
%\vspace{150mm}\\
%As long as all expressions involving $h_{\mu\nu}$ are converted to down indices, we need to take the conformal transformations of $\Omega^{-2}h_{\mu\nu}$. There is a problem in the program in the conformal weighting. With the above replacement, all terms $h_{\mu\nu}$ can be intrepreted at $\bar h_{\mu\nu}$ within the code. 
\newpage
\ba
	\delta R_{\mu\nu}&= \frac12 \del_\lambda \del^\lambda h_{\mu\nu}+\frac12 g^{\lambda\rho}\plr{ h^\sigma{}_\rho R_{\sigma \nu \mu \lambda}+h^\sigma{}_\rho R_{\sigma \mu \nu \lambda} - h^{\sigma}{}_\mu R_{\rho\sigma \nu \lambda} - h^\sigma{}_\nu R_{\rho\sigma\mu\lambda}}\\
	&\quad- \frac12\del_\nu \plr{ 4\Omega^{-1} \bar h^\rho{}_\mu  \pd_\rho \Omega - \Omega^{-1} h^\lambda{}_\lambda \pd_\mu \Omega} -\frac12\del_\mu \plr{4\Omega^{-1} \bar h^\rho{}_\nu  \pd_\rho \Omega - \Omega^{-1} h^\lambda{}_\lambda \pd_\nu \Omega}\\
\ea
\ba
	\frac12 \del_\lambda\del^\lambda h_{\mu\nu}&= \Omega^{-2}\plr{\frac12 \eta^{\alpha\beta}\pd_\beta\pd_\alpha h_{\mu\nu}}\\
	&\ +\Omega^{-3}\bigg( -\eta^{\alpha\beta}h_{\mu\nu}\pd_\beta\pd_\alpha\Omega - \eta^{\alpha\gamma}\pd_\alpha h_{\mu\nu}\pd_\gamma\Omega
	+ \eta^{\alpha\eta}\pd_\mu h_{\nu\alpha}\pd_\eta\Omega-\eta^{\alpha\beta}\pd_\beta h_{\nu\alpha}\pd_\mu\Omega\\
	&\qquad\qquad+\eta^{\alpha\lambda}\pd_\nu h_{\mu\alpha}\pd_\lambda\Omega - \eta^{\alpha\beta} \pd_\beta h_{\mu\alpha} \pd_\nu\Omega\bigg)\\
	&\ +\Omega^{-4}\bigg( \eta^{\alpha\eta}\eta^{\beta\rho}\eta_{\mu\nu} h_{\alpha\beta} \pd_\eta\Omega \pd_\rho\Omega -2 \eta^{\alpha\kappa}
	h_{\nu\alpha} \pd_\kappa\Omega \pd_\mu\Omega + \eta^{\alpha\beta} h_{\alpha\beta}\pd_\mu \Omega \pd_\nu \Omega - 2\eta^{\alpha\rho}h_{\mu\alpha}
	\pd_\nu \Omega\pd_\rho\Omega\bigg)
\ea
\ba
	\frac12 g^{\lambda\rho}(h^\sigma{}_\rho R_{\sigma \nu \mu \lambda}+h^\sigma{}_\rho R_{\sigma \mu \nu \lambda}&- h^{\sigma}{}_\mu R_{\rho\sigma \nu \lambda} - h^\sigma{}_\nu R_{\rho\sigma\mu\lambda})=\\
	&\quad\Omega^{-3}\bigg(\eta^{\alpha\beta}h_{\mu\nu} \pd_\beta\pd_\alpha \Omega +2\eta^{\alpha\beta} h_{\nu\alpha} \pd_\beta\pd_\mu\Omega +2
	\eta^{\alpha\beta}h_{\mu\alpha} \pd_\beta\pd_\nu \Omega\\
	&\qquad\qquad - \eta^{\alpha\beta}\eta^{\eta\gamma}\eta_{\mu\nu} h_{\alpha\gamma} \pd_\eta\pd_\beta \Omega
	-\eta^{\alpha\beta}h_{\alpha\beta}\pd_\nu\pd_\mu\Omega\bigg)\\
	&+\Omega^{-4}\bigg( -\eta^{\alpha\eta}\eta^{\gamma\beta}\eta_{\mu\nu}h_{\beta\gamma}\pd_\alpha\Omega\pd_\eta\Omega + 2\eta^{\alpha\kappa} h_{\mu\nu}\pd_\alpha\Omega
	\pd_\kappa\Omega\\
	&\qquad\qquad - 4 \eta^{\alpha\rho}h_{\nu\alpha}\pd_\rho \Omega \pd_\mu\Omega - 4\eta^{\alpha\eta}h_{\mu\alpha}\pd_\eta \Omega \pd_\nu\Omega 
	+2\eta^{\alpha\beta} h_{\alpha\beta}\pd_\mu\Omega \pd_\nu\Omega \\
	&\qquad\qquad+2\eta^{\alpha\lambda}\eta^{\beta\rho}\eta_{\mu\nu}h_{\alpha\beta}\pd_\lambda\Omega \pd_\rho\Omega\bigg)
\ea
\ba
	-\frac12\del_\nu \plr{ 4\Omega^{-1} \bar h^\rho{}_\mu  \pd_\rho \Omega - \Omega^{-1} h^\lambda{}_\lambda \pd_\mu \Omega}
	 &-\frac12\del_\mu \plr{4\Omega^{-1} \bar h^\rho{}_\nu  \pd_\rho \Omega - \Omega^{-1} h^\lambda{}_\lambda \pd_\nu \Omega}= \\
		 &\qquad\Omega^{-3}\plr{  2\eta^{\rho\kappa} \pd_\nu h_{\kappa\mu}\pd_\rho\Omega +2\eta^{\rho\kappa}h_{\kappa\mu} \pd_\nu\pd_\rho\Omega -\frac12 \eta^{\lambda\kappa}\pd_\nu
	 h_{\kappa\lambda}\pd_\mu\Omega - \frac12\eta^{\lambda\kappa}h_{\kappa\lambda}\pd_\nu\pd_\mu\Omega}\\
		 &\quad+\Omega^{-4}\bigg(\frac32 \eta^{\lambda\kappa}h_{\kappa\lambda}\pd_\nu\Omega\pd_\mu\Omega
		 +2\eta^{\rho\kappa}\eta^{\alpha\beta}\eta_{\mu\nu}h_{\kappa\alpha}\pd_\beta\Omega\pd_\rho\Omega-2\eta^{\rho\kappa}h_{\kappa\nu}\pd_\mu\Omega \pd_\rho\Omega\\
		 &\qquad\qquad\qquad -8\eta^{\rho\kappa}h_{\kappa\mu}\pd_\nu\Omega\pd_\rho\Omega  -\frac12\eta^{\lambda\kappa}\eta^{\alpha\beta}\eta_{\mu\nu}h_{\kappa\lambda}\pd_\alpha\Omega\pd_\beta\Omega\bigg)\\
		&\quad+(\mu\leftrightarrow\nu)
\ea
\\ \\
\[
	\frac12\Box\plr{ \Omega^{-2}\bar h_{\mu\nu}} = \frac12 \Omega^{-2}\Box \bar h_{\mu\nu} -\Omega^{-3}\bar h_{\mu\nu}\Box \Omega
\]\newpage
\ba
	\delta R_{\mu\nu}&= \frac12 \del_\lambda \del^\lambda h_{\mu\nu}+\frac12 g^{\lambda\rho}\plr{ h^\sigma{}_\rho R_{\sigma \nu \mu \lambda}+h^\sigma{}_\rho R_{\sigma \mu \nu \lambda} - h^{\sigma}{}_\mu R_{\rho\sigma \nu \lambda} - h^\sigma{}_\nu R_{\rho\sigma\mu\lambda}}\\
	&\quad- \frac12\del_\nu \plr{ 4\Omega^{-1} \bar h^\rho{}_\mu  \pd_\rho \Omega - \Omega^{-1} h^\lambda{}_\lambda \pd_\mu \Omega} -\frac12\del_\mu \plr{4\Omega^{-1} \bar h^\rho{}_\nu  \pd_\rho \Omega - \Omega^{-1} h^\lambda{}_\lambda \pd_\nu \Omega}\\
\ea
\ba
	\frac12 \del_\lambda\del^\lambda h_{\mu\nu}&= \frac12 g^{\lambda\rho}\{ \\
	&\quad[\pd_\lambda\pd_\rho - \Gamma^\sigma_{\lambda\rho}\pd_\sigma]h_{\mu\nu}
	+[\Gamma^\sigma_{\lambda\mu}\Gamma^{\kappa}_{\rho\nu}+\Gamma^\sigma_{\lambda\nu}\Gamma^\kappa_{\rho\mu}]h_{\kappa\sigma} + 
	[\Gamma^\sigma_{\lambda\nu}\Gamma^\kappa_{\rho\sigma} + \Gamma^\sigma_{\lambda\rho}\Gamma^\kappa_{\sigma\nu} - \pd_\lambda\Gamma^\kappa_{\rho\nu}
	-\Gamma^\kappa_{\rho\nu}\pd_\lambda - \Gamma^\kappa_{\lambda\nu}\pd_\rho]h_{\kappa\mu}\\
	&\quad+ [\Gamma^\sigma_{\lambda\mu}\Gamma^\kappa_{\rho\sigma} + \Gamma^\sigma_{\lambda\rho}\Gamma^\kappa_{\sigma\mu} - \pd_\lambda \Gamma^\kappa_{\rho\mu}
	-\Gamma^\kappa_{\rho\mu}\pd_\lambda - \Gamma^\kappa_{\lambda\mu}\pd_\rho]h_{\kappa\nu}\}
\ea
\ba
	\frac12 g^{\lambda\rho}(h^\sigma{}_\rho R_{\sigma \nu \mu \lambda})&=\frac12 g^{\lambda\rho}(h_{\sigma\rho} R^\sigma{}_{\nu \mu \lambda})\\
	&= \frac12 g^{\lambda\rho}[ \pd_\lambda\Gamma^\sigma_{\mu\nu} - \pd_\mu\Gamma^\sigma_{\lambda\nu} + \Gamma^\alpha_{\mu\nu}\Gamma^\sigma_{\lambda\alpha}
	-\Gamma^\alpha_{\lambda\nu}\Gamma^\sigma_{\mu\alpha}]h_{\sigma\rho}
\ea
\ba
	\frac12 g^{\lambda\rho}(h^\sigma{}_\rho R_{\sigma \nu \mu \lambda}+h^\sigma{}_\rho R_{\sigma \mu \nu \lambda}) &=
	\frac12 g^{\lambda\rho}[ 2\pd_\lambda\Gamma^\sigma_{\mu\nu} - \pd_\mu\Gamma^\sigma_{\lambda\nu}-\pd_\nu\Gamma^\sigma_{\lambda\mu}+2 \Gamma^\alpha_{\mu\nu}\Gamma^\sigma_{\lambda\alpha}
	-\Gamma^\alpha_{\lambda\nu}\Gamma^\sigma_{\mu\alpha}-\Gamma^\alpha_{\lambda\mu}\Gamma^\sigma_{\nu\alpha}]h_{\sigma\rho}
\ea
\ba
	\frac12 g^{\lambda\rho}(- h^{\sigma}{}_\mu R_{\rho\sigma \nu \lambda} )&= \frac12 g^{\lambda\rho}(h^{\sigma}{}_\mu R_{\sigma\rho \nu \lambda} )=\frac12 g^{\lambda\rho}( h_{\sigma\mu} R^\sigma{}_{\rho \nu \lambda} )\\
	&= \frac12 g^{\lambda\rho}[ \pd_\lambda\Gamma^\sigma_{\nu\rho} - \pd_\nu \Gamma^\sigma_{\lambda\rho} + \Gamma^\alpha_{\nu\rho}\Gamma^\sigma_{\lambda\alpha}
	- \Gamma^\alpha_{\lambda\rho}\Gamma^\sigma_{\nu\alpha}]h_{\sigma\mu}
\ea
\ba
	\frac12 g^{\lambda\rho}(- h^{\sigma}{}_\nu R_{\rho\sigma \mu \lambda} )
	&= \frac12 g^{\lambda\rho}[ \pd_\lambda\Gamma^\sigma_{\mu\rho} - \pd_\mu \Gamma^\sigma_{\lambda\rho} + \Gamma^\alpha_{\mu\rho}\Gamma^\sigma_{\lambda\alpha}
	- \Gamma^\alpha_{\lambda\rho}\Gamma^\sigma_{\mu\alpha}]h_{\sigma\nu}
\ea
\ba
	\frac12 g^{\lambda\rho}(h^\sigma{}_\rho R_{\sigma \nu \mu \lambda}+h^\sigma{}_\rho R_{\sigma \mu \nu \lambda}&- h^{\sigma}{}_\mu R_{\rho\sigma \nu \lambda} - h^\sigma{}_\nu R_{\rho\sigma\mu\lambda})=\frac12 g^{\lambda\rho}\big\{ \\
	&\ \quad [ 2\pd_\lambda\Gamma^\sigma_{\mu\nu} - \pd_\mu\Gamma^\sigma_{\lambda\nu}-\pd_\nu\Gamma^\sigma_{\lambda\mu}+2 \Gamma^\alpha_{\mu\nu}\Gamma^\sigma_{\lambda\alpha}
	-\Gamma^\alpha_{\lambda\nu}\Gamma^\sigma_{\mu\alpha}-\Gamma^\alpha_{\lambda\mu}\Gamma^\sigma_{\nu\alpha}]h_{\sigma\rho}\\
	&+ [ \pd_\lambda\Gamma^\sigma_{\nu\rho} - \pd_\nu \Gamma^\sigma_{\lambda\rho} + \Gamma^\alpha_{\nu\rho}\Gamma^\sigma_{\lambda\alpha}
	- \Gamma^\alpha_{\lambda\rho}\Gamma^\sigma_{\nu\alpha}]h_{\sigma\mu}\\
	&+[ \pd_\lambda\Gamma^\sigma_{\mu\rho} - \pd_\mu \Gamma^\sigma_{\lambda\rho} + \Gamma^\alpha_{\mu\rho}\Gamma^\sigma_{\lambda\alpha}
	- \Gamma^\alpha_{\lambda\rho}\Gamma^\sigma_{\mu\alpha}]h_{\sigma\nu} \big\}
\ea
\ba
	-\frac12\del_\nu \plr{ 4\Omega^{-1} \bar h^\rho{}_\mu  \pd_\rho \Omega - \Omega^{-1} h^\lambda{}_\lambda \pd_\mu \Omega}
	 &-\frac12\del_\mu \plr{4\Omega^{-1} \bar h^\rho{}_\nu  \pd_\rho \Omega - \Omega^{-1} h^\lambda{}_\lambda \pd_\nu \Omega}= \\
		 &\qquad\Omega^{-3}\plr{  2\eta^{\rho\kappa} \pd_\nu h_{\kappa\mu}\pd_\rho\Omega +2\eta^{\rho\kappa}h_{\kappa\mu} \pd_\nu\pd_\rho\Omega -\frac12 \eta^{\lambda\kappa}\pd_\nu
	 h_{\kappa\lambda}\pd_\mu\Omega - \frac12\eta^{\lambda\kappa}h_{\kappa\lambda}\pd_\nu\pd_\mu\Omega}\\
		 &\quad+\Omega^{-4}\bigg(\frac32 \eta^{\lambda\kappa}h_{\kappa\lambda}\pd_\nu\Omega\pd_\mu\Omega
		 +2\eta^{\rho\kappa}\eta^{\alpha\beta}\eta_{\mu\nu}h_{\kappa\alpha}\pd_\beta\Omega\pd_\rho\Omega-2\eta^{\rho\kappa}h_{\kappa\nu}\pd_\mu\Omega \pd_\rho\Omega\\
		 &\qquad\qquad\qquad -8\eta^{\rho\kappa}h_{\kappa\mu}\pd_\nu\Omega\pd_\rho\Omega  -\frac12\eta^{\lambda\kappa}\eta^{\alpha\beta}\eta_{\mu\nu}h_{\kappa\lambda}\pd_\alpha\Omega\pd_\beta\Omega\bigg)\\
		&\quad+(\mu\leftrightarrow\nu)
\ea
\\ \\
\[
	\frac12\Box\plr{ \Omega^{-2}\bar h_{\mu\nu}} = \frac12 \Omega^{-2}\Box \bar h_{\mu\nu} -\Omega^{-3}\bar h_{\mu\nu}\Box \Omega
\]
\\ 
\newpage
Gauge: 
\[
	 \bar \del_\mu \bar h^\mu{}_\nu = \frac12 \bar \del_\nu \bar h^\mu{}_\mu  + \bar \Gamma^\mu_{\mu\rho} \bar h^\rho{}_\nu - \bar\Gamma^\rho_{\mu\nu} \bar h^{\mu}{}_\rho
\]
\ba
	\delta R_{\mu\nu}&= \frac12 \del_\lambda \del^\lambda h_{\mu\nu}+\frac12 g^{\lambda\rho}\plr{ h^\sigma{}_\rho R_{\sigma \nu \mu \lambda}+h^\sigma{}_\rho R_{\sigma \mu \nu \lambda} - h^{\sigma}{}_\mu R_{\rho\sigma \nu \lambda} - h^\sigma{}_\nu R_{\rho\sigma\mu\lambda}}\\
	&\quad+\frac12 \del_\mu (\Gamma^\sigma_{\rho\nu}h^\rho{}_\sigma - \Gamma^\sigma_{\sigma\rho}h^\rho{}_\nu)+\frac12 \del_\nu (
	\Gamma^\sigma_{\rho\mu}h^\rho{}_\sigma - \Gamma^\sigma_{\sigma\rho}h^\rho{}_\mu)
\ea
\ba
	\frac12 \del_\lambda\del^\lambda h_{\mu\nu}&= \frac12 g^{\lambda\rho}\{ \\
	&\quad[\pd_\lambda\pd_\rho - \Gamma^\sigma_{\lambda\rho}\pd_\sigma]h_{\mu\nu}
	+[\Gamma^\sigma_{\lambda\mu}\Gamma^{\kappa}_{\rho\nu}+\Gamma^\sigma_{\lambda\nu}\Gamma^\kappa_{\rho\mu}]h_{\kappa\sigma} + 
	[\Gamma^\sigma_{\lambda\nu}\Gamma^\kappa_{\rho\sigma} + \Gamma^\sigma_{\lambda\rho}\Gamma^\kappa_{\sigma\nu} - \pd_\lambda\Gamma^\kappa_{\rho\nu}
	-\Gamma^\kappa_{\rho\nu}\pd_\lambda - \Gamma^\kappa_{\lambda\nu}\pd_\rho]h_{\kappa\mu}\\
	&\quad+ [\Gamma^\sigma_{\lambda\mu}\Gamma^\kappa_{\rho\sigma} + \Gamma^\sigma_{\lambda\rho}\Gamma^\kappa_{\sigma\mu} - \pd_\lambda \Gamma^\kappa_{\rho\mu}
	-\Gamma^\kappa_{\rho\mu}\pd_\lambda - \Gamma^\kappa_{\lambda\mu}\pd_\rho]h_{\kappa\nu}\}
\ea
\ba
	\frac12 g^{\lambda\rho}(h^\sigma{}_\rho R_{\sigma \nu \mu \lambda}+h^\sigma{}_\rho R_{\sigma \mu \nu \lambda}&- h^{\sigma}{}_\mu R_{\rho\sigma \nu \lambda} - h^\sigma{}_\nu R_{\rho\sigma\mu\lambda})=\frac12 g^{\lambda\rho}\big\{ \\
	&\ \quad [ 2\pd_\lambda\Gamma^\sigma_{\mu\nu} - \pd_\mu\Gamma^\sigma_{\lambda\nu}-\pd_\nu\Gamma^\sigma_{\lambda\mu}+2 \Gamma^\alpha_{\mu\nu}\Gamma^\sigma_{\lambda\alpha}
	-\Gamma^\alpha_{\lambda\nu}\Gamma^\sigma_{\mu\alpha}-\Gamma^\alpha_{\lambda\mu}\Gamma^\sigma_{\nu\alpha}]h_{\sigma\rho}\\
	&+ [ \pd_\lambda\Gamma^\sigma_{\nu\rho} - \pd_\nu \Gamma^\sigma_{\lambda\rho} + \Gamma^\alpha_{\nu\rho}\Gamma^\sigma_{\lambda\alpha}
	- \Gamma^\alpha_{\lambda\rho}\Gamma^\sigma_{\nu\alpha}]h_{\sigma\mu}\\
	&+[ \pd_\lambda\Gamma^\sigma_{\mu\rho} - \pd_\mu \Gamma^\sigma_{\lambda\rho} + \Gamma^\alpha_{\mu\rho}\Gamma^\sigma_{\lambda\alpha}
	- \Gamma^\alpha_{\lambda\rho}\Gamma^\sigma_{\mu\alpha}]h_{\sigma\nu} \big\}
\ea
\ba
	\frac12 \del_\lambda\del^\lambda h_{\mu\nu}&+\frac12 g^{\lambda\rho}(h^\sigma{}_\rho R_{\sigma \nu \mu \lambda}+h^\sigma{}_\rho R_{\sigma \mu \nu \lambda}- h^{\sigma}{}_\mu R_{\rho\sigma \nu \lambda} - h^\sigma{}_\nu R_{\rho\sigma\mu\lambda})\\
	&=\frac12 g^{\lambda\rho}\big\{ [\pd_\lambda\pd_\rho - \Gamma^\sigma_{\lambda\rho}\pd_\sigma]h_{\mu\nu}+[\Gamma^\sigma_{\lambda\mu}\Gamma^{\kappa}_{\rho\nu}
	+\Gamma^\sigma_{\lambda\nu}\Gamma^\kappa_{\rho\mu}]h_{\kappa\sigma} \\
	&\qquad\quad + [ 2\pd_\lambda\Gamma^\sigma_{\mu\nu} - \pd_\mu\Gamma^\sigma_{\lambda\nu}-\pd_\nu\Gamma^\sigma_{\lambda\mu}+2 \Gamma^\alpha_{\mu\nu}\Gamma^\sigma_{\lambda\alpha}
	-\Gamma^\alpha_{\lambda\nu}\Gamma^\sigma_{\mu\alpha}-\Gamma^\alpha_{\lambda\mu}\Gamma^\sigma_{\nu\alpha}]h_{\sigma\rho}\\
	&\qquad\quad+ [  - \pd_\nu \Gamma^\sigma_{\lambda\rho} + 2\Gamma^\alpha_{\nu\rho}\Gamma^\sigma_{\lambda\alpha}-\Gamma^\sigma_{\rho\nu}\pd_\lambda - \Gamma^\sigma_{\lambda\nu}\pd_\rho]h_{\sigma\mu}\\
	&\qquad\quad+ [  - \pd_\mu \Gamma^\sigma_{\lambda\rho} + 2\Gamma^\alpha_{\mu\rho}\Gamma^\sigma_{\lambda\alpha}-\Gamma^\sigma_{\rho\mu}\pd_\lambda - \Gamma^\sigma_{\lambda\mu}\pd_\rho]h_{\sigma\nu}\big\}\\
\ea
\ba
	\frac12\del_\mu( \Gamma^\sigma_{\rho\nu}h^\rho{}_\sigma - \Gamma^\sigma_{\sigma\rho}h^\rho{}_\nu) = \frac12 g^{\lambda\rho}\del_\mu (\Gamma^\sigma_{\rho\nu}
	h_{\lambda\sigma} - \Gamma^\rho_{\rho\sigma}h_{\lambda\nu})
\ea
\ba
	 \frac12 g^{\lambda\rho}\del_\mu (\Gamma^\sigma_{\rho\nu}h_{\lambda\sigma})  &= \frac12 g^{\lambda\rho} (h_{\lambda\sigma}\del_\mu \Gamma^\sigma_{\rho\nu} 
	+ \Gamma^\sigma_{\rho\nu} \del_\mu h_{\lambda\sigma})
\ea
\ba
	\del_\mu( \Gamma^\sigma_{\rho\nu}h^\rho{}_\sigma ) &\equiv \del_\mu T_{\nu} = \pd_\mu T_\nu - \Gamma^\lambda_{\mu\nu}T_\lambda\\
	&=\pd_\mu \Gamma^\sigma_{\rho\nu}h^\rho{}_\sigma -\Gamma^\lambda_{\mu\nu} \Gamma^\sigma_{\rho\lambda}h^\rho{}_\sigma
\ea
\newpage\noindent
Gauge: 
\[
	 \bar \del_\mu \bar h^\mu{}_\nu = \frac12 \bar \del_\nu \bar h^\mu{}_\mu  + \bar \Gamma^\mu_{\mu\rho} \bar h^\rho{}_\nu - \bar\Gamma^\rho_{\mu\nu} \bar h^{\mu}{}_\rho
\]
We can also write this as:
\[
	 \bar \del_\mu \bar h^\mu{}_\nu = \frac12 \bar \del_\nu \bar h^\mu{}_\mu  + (\bar \del_\mu-\pd_\mu)\bar h^\mu{}_\nu
\]
\ba
	\delta R_{\mu\nu}&= \frac12 \del_\lambda \del^\lambda h_{\mu\nu}+\frac12 g^{\lambda\rho}\plr{ h^\sigma{}_\rho R_{\sigma \nu \mu \lambda}+h^\sigma{}_\rho R_{\sigma \mu \nu \lambda} - h^{\sigma}{}_\mu R_{\rho\sigma \nu \lambda} - h^\sigma{}_\nu R_{\rho\sigma\mu\lambda}}\\
	&\quad+\frac12 \del_\mu (\Gamma^\sigma_{\rho\nu}h^\rho{}_\sigma - \Gamma^\sigma_{\sigma\rho}h^\rho{}_\nu)+\frac12 \del_\nu (
	\Gamma^\sigma_{\rho\mu}h^\rho{}_\sigma - \Gamma^\sigma_{\sigma\rho}h^\rho{}_\mu)
\ea

\ba
	\frac12 \del_\lambda\del^\lambda h_{\mu\nu}&+\frac12 g^{\lambda\rho}(h^\sigma{}_\rho R_{\sigma \nu \mu \lambda}+h^\sigma{}_\rho R_{\sigma \mu \nu \lambda}- h^{\sigma}{}_\mu R_{\rho\sigma \nu \lambda} - h^\sigma{}_\nu R_{\rho\sigma\mu\lambda})\\
	&=\frac12 g^{\lambda\rho}\big\{ [\pd_\lambda\pd_\rho - \Gamma^\sigma_{\lambda\rho}\pd_\sigma]h_{\mu\nu}+[\Gamma^\sigma_{\lambda\mu}\Gamma^{\kappa}_{\rho\nu}
	+\Gamma^\sigma_{\lambda\nu}\Gamma^\kappa_{\rho\mu}]h_{\kappa\sigma} \\
	&\qquad\quad + [ 2\pd_\lambda\Gamma^\sigma_{\mu\nu} - \pd_\mu\Gamma^\sigma_{\lambda\nu}-\pd_\nu\Gamma^\sigma_{\lambda\mu}+2 \Gamma^\alpha_{\mu\nu}\Gamma^\sigma_{\lambda\alpha}
	-\Gamma^\alpha_{\lambda\nu}\Gamma^\sigma_{\mu\alpha}-\Gamma^\alpha_{\lambda\mu}\Gamma^\sigma_{\nu\alpha}]h_{\sigma\rho}\\
	&\qquad\quad+ [  - \pd_\nu \Gamma^\sigma_{\lambda\rho} + 2\Gamma^\alpha_{\nu\rho}\Gamma^\sigma_{\lambda\alpha}-\Gamma^\sigma_{\rho\nu}\pd_\lambda - \Gamma^\sigma_{\lambda\nu}\pd_\rho]h_{\sigma\mu}\\
	&\qquad\quad+ [  - \pd_\mu \Gamma^\sigma_{\lambda\rho} + 2\Gamma^\alpha_{\mu\rho}\Gamma^\sigma_{\lambda\alpha}-\Gamma^\sigma_{\rho\mu}\pd_\lambda - \Gamma^\sigma_{\lambda\mu}\pd_\rho]h_{\sigma\nu}\big\}
\ea

\ba
	\frac12 \del_\mu (\Gamma^\sigma_{\rho\nu}h^\rho{}_\sigma - \Gamma^\sigma_{\sigma\rho}h^\rho{}_\nu) &=  \frac12g^{\lambda\rho}\blr{ 
	(\pd_\mu \Gamma^\sigma_{\lambda\nu}+\Gamma^\sigma_{\lambda\nu}\pd_\mu  - \Gamma^\kappa_{\mu\nu}\Gamma^\sigma_{\lambda\kappa}+ \Gamma^\sigma_{\mu\nu}\Gamma^\kappa_{\kappa\lambda})h_{\sigma\rho} 
	- (\pd_\mu\Gamma^\sigma_{\sigma\lambda}+ \Gamma^\sigma_{\sigma\lambda}\pd_\mu)h_{\rho\nu}}  \\
	&\quad +\frac12 \pd_\mu g^{\lambda\rho} \plr{ \Gamma^\sigma_{\lambda\nu} h_{\rho\sigma} - \Gamma^\sigma_{\sigma\lambda} h_{\rho\nu}}
\ea
\\ \\ \\
\[
	\Gamma^\sigma_{\rho\nu} h^\rho{}_\sigma = \Omega^{-1} h^\sigma{}_\sigma \del_\nu \Omega
\]
\[
	\Gamma^\sigma_{\sigma\rho}h^\rho{}_\nu= 4\Omega^{-1} h^\rho{}_\nu \del_\rho \Omega
\]
\ba
	\del_\mu( \Gamma^\sigma_{\rho\nu}h^\rho{}_\sigma ) &\equiv \del_\mu T_{\nu} = \pd_\mu T_\nu - \Gamma^\lambda_{\mu\nu}T_\lambda\\
	&=\pd_\mu( \Gamma^\sigma_{\rho\nu}h^\rho{}_\sigma) -\Gamma^\lambda_{\mu\nu} \Gamma^\sigma_{\rho\lambda}h^\rho{}_\sigma
\ea

\vspace{500mm}
\ba
	\del_\mu( \Gamma^\sigma_{\rho\nu}h^\rho{}_\sigma ) &\equiv \del_\mu T_{\nu} = \pd_\mu T_\nu - \Gamma^\lambda_{\mu\nu}T_\lambda\\
	&=\pd_\mu( \Gamma^\sigma_{\rho\nu}h^\rho{}_\sigma) -\Gamma^\lambda_{\mu\nu} \Gamma^\sigma_{\rho\lambda}h^\rho{}_\sigma
\ea

\ba
	\frac12 \del_\mu(\del_\rho-\pd_\rho)h^\rho{}_\nu = \frac12 g^{\lambda\rho}[\del_\mu \del_\rho h_{\lambda\nu}- \del_\mu(\pd_\rho g^{\lambda\rho}h_{\lambda\nu})]
\ea
\ba
	\delta R_{\mu\nu}&= \frac12 \del_\lambda \del^\lambda h_{\mu\nu}+\frac12 g^{\lambda\rho}\plr{ h^\sigma{}_\rho R_{\sigma \nu \mu \lambda}+h^\sigma{}_\rho R_{\sigma \mu \nu \lambda} - h^{\sigma}{}_\mu R_{\rho\sigma \nu \lambda} - h^\sigma{}_\nu R_{\rho\sigma\mu\lambda}}\\
	&\quad-\frac12 \del_\mu (\del_\lambda-\pd_\lambda)h^\lambda{}_\nu-\frac12 \del_\nu (\del_\lambda-\pd_\lambda)h^\lambda{}_\mu
\ea
\ba
	\delta R_{\mu\nu}&= \frac12 (\del_\lambda \del^\lambda h_{\mu\nu}- \del_\lambda \del_\mu h^\lambda{}_\nu-\del_\lambda \del_\nu h^\lambda{}_\mu) - \del_\mu\pd_\lambda h^\lambda{}_\nu - \del_\nu\pd_\lambda h^\lambda{}_\mu
\ea
\[
	\Gamma^\sigma_{\rho\nu} h^\rho{}_\sigma = \Omega^{-1} h^\sigma{}_\sigma \del_\nu \Omega
\]
\[
	\Gamma^\sigma_{\sigma\rho}h^\rho{}_\nu= 4\Omega^{-1} h^\rho{}_\nu \del_\rho \Omega
\]
\ba
	\frac12 \del_\mu (\Gamma^\sigma_{\rho\nu}h^\rho{}_\sigma - \Gamma^\sigma_{\sigma\rho}h^\rho{}_\nu) &= \frac12\blr{ 
	\pd_\mu (\Gamma^\sigma_{\rho\nu}h^\rho{}_\sigma) - \Gamma^\kappa_{\mu\nu}\Gamma^\sigma_{\rho\kappa}h^\rho{}_\sigma
	- \pd_\mu(\Gamma^\sigma_{\sigma\rho}h^\rho{}_\nu) + \Gamma^\kappa_{\mu\nu}\Gamma^\sigma_{\sigma\rho}h^\rho{}_\kappa }\\
	&= \frac12\blr{ 
	(\pd_\mu \Gamma^\sigma_{\rho\nu}+\Gamma^\sigma_{\rho\nu}\pd_\mu  - \Gamma^\kappa_{\mu\nu}\Gamma^\sigma_{\rho\kappa})h^{\rho}{}_{\sigma} 
	- (\pd_\mu\Gamma^\sigma_{\sigma\rho}+ \Gamma^\sigma_{\sigma\rho}\pd_\mu)h^\rho{}_\nu  + \Gamma^\kappa_{\mu\nu}\Gamma^\sigma_{\sigma\rho}h^\rho{}_\kappa }\\
	&=  \frac12g^{\lambda\rho}\blr{ 
	(\pd_\mu \Gamma^\sigma_{\rho\nu}+\Gamma^\sigma_{\rho\nu}\pd_\mu  - \Gamma^\kappa_{\mu\nu}\Gamma^\sigma_{\rho\kappa})h_{\lambda\sigma} 
	- (\pd_\mu\Gamma^\sigma_{\sigma\rho}+ \Gamma^\sigma_{\sigma\rho}\pd_\mu)h_{\lambda\nu}  + \Gamma^\kappa_{\mu\nu}\Gamma^\sigma_{\sigma\rho}h_{\lambda\kappa }}\\
	&\quad +\frac12 \pd_\mu g^{\lambda\rho} \plr{ \Gamma^\sigma_{\rho\nu} h_{\lambda\sigma} - \Gamma^\sigma_{\sigma\rho} h_{\lambda\nu}}\\
	&=  \frac12g^{\lambda\rho}\blr{ 
	(\pd_\mu \Gamma^\sigma_{\lambda\nu}+\Gamma^\sigma_{\lambda\nu}\pd_\mu  - \Gamma^\kappa_{\mu\nu}\Gamma^\sigma_{\lambda\kappa}+ \Gamma^\sigma_{\mu\nu}\Gamma^\kappa_{\kappa\lambda})h_{\sigma\rho} 
	- (\pd_\mu\Gamma^\sigma_{\sigma\lambda}+ \Gamma^\sigma_{\sigma\lambda}\pd_\mu)h_{\rho\nu}}  \\
	&\quad +\frac12 \pd_\mu g^{\lambda\rho} \plr{ \Gamma^\sigma_{\lambda\nu} h_{\rho\sigma} - \Gamma^\sigma_{\sigma\lambda} h_{\rho\nu}}
\ea
$ ds^2 = -(1+2\phi)d\tau^2 + (B_i + \nabla_i B)dx^i d\tau + [(1-2\psi)\delta_{ij} + 2[ (\nabla_i \nabla_j - 1/3 \nabla^2)E + 1/2( \nabla_i E_j + \nabla_j E_i) + E_{ij}]]dx^i dx^j $
\end{document}