\documentclass[10pt,letterpaper]{article}
\usepackage[textwidth=7in, top=1in,textheight=9in]{geometry}
\usepackage[fleqn]{mathtools} 
\usepackage{amssymb,braket,hyperref,xcolor}
\hypersetup{colorlinks, linkcolor={blue!50!black}, citecolor={red!50!black}, urlcolor={blue!80!black}}
\usepackage[title]{appendix}
\usepackage[sorting=none]{biblatex}
\numberwithin{equation}{section}
\setlength{\parindent}{0pt}
\title{RW SVT4 Decomposition v1}
\date{}
\allowdisplaybreaks
\begin{document} 
\maketitle
\noindent 
%%%%%%%%%%%%%%%%%%%%%%%%%%%%%%%%
\section{Background}
%%%%%%%%%%%%%%%%%%%%%%%%%%%%%%%%%%
\begin{eqnarray}
ds^2 &=& \Omega^2(\tau)\left(-d\tau^2 +\tilde g_{ij} dx^i dx^j\right),\qquad R_{ij} = -2k \tilde g_{ij}
\label{geom2}
\\ \nonumber\\
R_{\lambda\mu\nu\kappa} &=&- \tfrac{1}{6} g_{\lambda \nu } g_{\mu \kappa } R + \tfrac{1}{6} g_{\lambda \kappa } g_{\mu \nu } R -  \tfrac{1}{2} g_{\mu \nu } R_{\lambda \kappa } + \tfrac{1}{2} g_{\mu \kappa } R_{\lambda \nu } + \tfrac{1}{2} g_{\lambda \nu } R_{\mu \kappa } -  \tfrac{1}{2} g_{\lambda \kappa } R_{\mu \nu }
\\ \nonumber\\
R_{\mu\nu} &=& (A+B)U_\mu U_\nu + g_{\mu\nu}B,\qquad R=3B-A
\label{Ricci}
\\ \nonumber\\
A &=& -\tfrac12 (3p+\rho)
\nonumber\\
&=& -3 \dot{\Omega}^2 \Omega^{-4} + 3 \overset{..}{\Omega} \Omega^{-3}
\\ \nonumber\\
B&=& \tfrac12(p-\rho)
\nonumber\\
&=& - \dot{\Omega}^2 \Omega^{-4} -  \overset{..}{\Omega} \Omega^{-3} - 2 k \Omega^{-2}
\\ \nonumber\\
\rho &=& \tfrac{1}{2} (- A - 3 B)
\nonumber\\
&=& 3 \dot{\Omega}^2 \Omega^{-4} + 3 k \Omega^{-2}
\\ \nonumber\\
p &=& \tfrac{1}{2} (- A + B)
\nonumber\\
&=& \dot{\Omega}^2 \Omega^{-4} - 2 \overset{..}{\Omega} \Omega^{-3} -  k \Omega^{-2}
\end{eqnarray}
%
%
%%%%%%%%%%%%%%%%%
\subsection{Identities}
%%%%%%%%%%%%%%%%%
$A, B, \rho, p$ are functions only of coordinate $x^0$. 
\begin{eqnarray}
U^\alpha U^\beta \nabla_\alpha F\nabla_\beta A &=& -\nabla^\alpha F \nabla_\alpha A
\\ \nonumber\\
F^\alpha U_\alpha U^\beta \nabla_\beta A &=& -F^\alpha \nabla_\alpha A
\\ \nonumber\\
U^\alpha\nabla_\alpha U^\mu &=& 0
\\ \nonumber\\
\nabla_\mu U_\nu &=& \dot\Omega \Omega^{-2}(g_{\mu\nu} + U_{\mu}U_\nu)
\end{eqnarray}
%
%
\newpage
%%%%%%%%%%%%%%%%%%%%%%%%%%
\section{Fluctuations}
%%%%%%%%%%%%%%%%%%%%%%%%%%
%
%
\begin{eqnarray}
ds^2 &=& ( g_{\mu\nu}+ h_{\mu\nu}) dx^\mu dx^\nu
\\ \nonumber\\
g^{\mu\nu} F_{\mu\nu} &=&0,\qquad \nabla^\mu F_{\mu\nu} = 0,\qquad \nabla^\mu F_\mu=0 
\\ \nonumber\\
h_{\mu\nu} &=& -2 g_{\mu\nu}\chi + 2\nabla_\mu \nabla_\nu F +\nabla_\mu F_\nu +\nabla_\nu F_\mu+ 2F_{\mu\nu}
\label{svt}
\\ \nonumber\\
g^{\alpha\beta}h_{\alpha\beta} &=& -8\chi +2 \nabla_\alpha \nabla^\alpha F
\\ \nonumber\\
\nabla^\mu h_{\mu\nu} &=& 2 U^{\alpha } U_{\nu } (p + \rho) \nabla_{\alpha }F + (- p + \rho) \nabla_{\nu }F - 2 \nabla_{\nu }\chi + 2 \nabla_{\nu }\nabla_{\alpha }\nabla^{\alpha }F+\tfrac{1}{2} F_{\nu } (- p + \rho) \nonumber \\ 
&& + F^{\alpha } U_{\alpha } U_{\nu } (p + \rho) + \nabla_{\alpha }\nabla^{\alpha }F_{\nu }
\\ \nonumber\\
\nabla^\mu \nabla^\nu h_{\mu\nu} &=&  (- p + \rho) \nabla_{\alpha }\nabla^{\alpha }F - 2 \nabla_{\alpha }\nabla^{\alpha }\chi + (-3 \nabla_{\alpha }p -  \nabla_{\alpha }\rho) \nabla^{\alpha }F + 2 U^{\alpha } (p + \rho) \nabla_{\alpha }F \nabla_{\beta }U^{\beta } \nonumber \\ 
&& + 2 U^{\alpha } U^{\beta } (p + \rho) \nabla_{\beta }\nabla_{\alpha }F + 2 \nabla_{\beta }\nabla^{\beta }\nabla_{\alpha }\nabla^{\alpha }F+2 U^{\alpha } U^{\beta } (p + \rho) \nabla_{\beta }F_{\alpha } \nonumber \\ 
&& + F^{\alpha } \bigl(-3 \nabla_{\alpha }p -  \nabla_{\alpha }\rho + 2 U_{\alpha } (p + \rho) \nabla_{\beta }U^{\beta }\bigr)
\\ \nonumber\\
U^\mu U^\nu h_{\mu\nu} &=& 2 \chi + 2 U^{\alpha } U^{\beta } \nabla_{\beta }\nabla_{\alpha }F+2 U^{\alpha } U^{\beta } \nabla_{\beta }F_{\alpha }+2 F_{\alpha \beta } U^{\alpha } U^{\beta }
\\ \nonumber\\
(U^\mu U^\nu +g^{\mu\nu})h_{\mu\nu} &=& -6 \chi + 2 \nabla_{\alpha }\nabla^{\alpha }F + 2 U^{\alpha } U^{\beta } \nabla_{\beta }\nabla_{\alpha }F+2 U^{\alpha } U^{\beta } \nabla_{\beta }F_{\alpha }+2 F_{\alpha \beta } U^{\alpha } U^{\beta }
\\ \nonumber\\
(U^\mu \nabla^\nu + U^\nu \nabla^\mu)h_{\mu\nu} &=& -4 U^{\alpha } \nabla_{\alpha }\chi + 4 U^{\alpha } \nabla_{\beta }\nabla^{\beta }\nabla_{\alpha }F- F^{\alpha } U_{\alpha } (3 p + \rho) + 2 U^{\alpha } \nabla_{\beta }\nabla^{\beta }F_{\alpha }
\end{eqnarray}
\\ \\
\begin{eqnarray}
\Delta_{\mu\nu}'&=& 2 (p + \rho) U_{\mu } U_{\nu } U^{\alpha } \nabla_{\alpha }V^{GI}{} + (\tfrac{2}{3} g_{\mu \nu } + \tfrac{2}{3} U_{\mu } U_{\nu }) \nabla_{\alpha }\nabla^{\alpha }\chi + (\tfrac{2}{3} g_{\mu \nu } U^{\alpha } U^{\beta } + \tfrac{8}{3} U_{\mu } U_{\nu } U^{\alpha } U^{\beta }) \nabla_{\beta }\nabla_{\alpha }\chi \nonumber \\ 
&& + (p + \rho) U_{\nu } \nabla_{\mu }V^{GI}{} + (p + \rho) U_{\mu } \nabla_{\nu }V^{GI}{} - 2 \nabla_{\nu }\nabla_{\mu }\chi +2 (p + \rho) U_{\mu } U_{\nu } U^{\alpha } V_{\alpha } + (p + \rho) U_{\nu } V_{\mu } \nonumber \\ 
&& + (p + \rho) U_{\mu } V_{\nu }+\bigl(\tfrac{2}{9} \rho g_{\mu \nu } U^{\alpha } U^{\beta } -  \tfrac{4}{9} (9 p + 7 \rho) U_{\mu } U_{\nu } U^{\alpha } U^{\beta }\bigr) F_{\alpha \beta } - 2 (p + \rho) U_{\nu } U^{\alpha } F_{\mu \alpha } -  \tfrac{2}{3} \rho F_{\mu \nu } \nonumber \\ 
&& - 2 (p + \rho) U_{\mu } U^{\alpha } F_{\nu \alpha } + \nabla_{\alpha }\nabla^{\alpha }F_{\mu \nu } + (- \tfrac{1}{3} g_{\mu \nu } U^{\alpha } U^{\beta } -  \tfrac{4}{3} U_{\mu } U_{\nu } U^{\alpha } U^{\beta }) \nabla_{\gamma }\nabla^{\gamma }F_{\alpha \beta }
\end{eqnarray}
\end{document}