\documentclass[9pt,letterpaper]{article}
\usepackage[top=1in,textheight=9in,margin=1.5in]{geometry}
\usepackage{mathtools}
\usepackage{setspace}
\usepackage{braket}
\usepackage{enumitem}
\usepackage{hyperref}
\newcommand{\vect}[1]{\mathbf{#1}}
\newcommand{\vecth}[1]{\hat{\mathbf{#1}}}
\newcommand{\h}{\hbar}
\newcommand{\epo}{\epsilon_0}
\newcommand{\pder}[2][]{\frac{\partial#1}{\partial#2}}

\title{Identities and Formulas in Quantum Mechanics}
\author{Matthew Phelps}
\date{Updated: \today}

\begin{document}
\begin{align*}W_{int} &= k\sum_{i=1}^n\sum_{j<i}{\frac{q_iq_j}{|\vect x_i-\vect x_j|}}=\frac k2\sum_i^n\sum_{\substack{j\\j\neq i}}\frac{q_iq_j}{|\vect x_i-\vect x_j|}=\frac{1}{2}\sum_{i=1}^nq_i\sum_{\substack{j\\j\neq i}}k\frac{q_j}{|\vect x_i-\vect x_j|}\\
&=\frac 12\sum_{i=1}^nq_i\Phi(\vect x_i)=\frac 12\int_\rho{\rho(\vect x)\Phi(\vect x)\,d^3x}=\frac \epo2\int_{all}{|\vect E|^2\,d^3x}=-\int_\infty^r{\vect F\cdot d\vect l}=\frac 12 q\Phi_*(\vect x)
\end{align*}
$$W_{int\text -dip} = \vect p\cdot\vect E;\quad W_{12} = \frac{\vect p_1\cdot\vect p_2-3(\vect n\cdot \vect p_1)(\vect n\cdot\vect p_2)}{4\pi\epo|\vect x_1-\vect x_2|^3}\quad\text{where}\quad \vect x_1\neq\vect x_2\quad \vect n = \frac{\vect x_1-\vect x_2}{|\vect x_1-\vect x_2|}$$
$$\Phi_{dipole\text-o}(\vect r)=k\frac{\vect p\cdot\vect r}{r^3};\quad \vect F_{dip} = (\vect p\cdot\nabla)\vect E;\quad W_{intqsp}=\frac{q^2}{2C};\quad -kq^2/2z\quad -k/2q^2R/(r^2-R^2)$$
$$\quad \vect E_{dip}(\vect x) = k\left(\frac{3\vect n(\vect p\cdot\vect n)-\vect p}{|\vect x-\vect x_0|^3}-\frac{4\pi}{3}\vect p\delta(\vect x-\vect x_0)\right)\quad\text{where}\quad \vect n=\frac{\vect x-\vect x_0}{|\vect x-\vect x_0|}$$
$$\Phi(\vect x)\approx k\left(\frac{1}{r}\int{\rho(\vect x')\,d^3x'}+\frac{\vect p\cdot\vect x}{r^3}\right)\quad\text{for}\quad r>r';\quad\vect p = \int{\vect x'\rho(\vect x')\,d^3x'}$$
$$\nabla = \pder r\vecth r+\frac 1r\pder\theta\vecth\theta+\frac{1}{r\sin\theta}\pder\phi\vecth\phi;\quad-\nabla_x\left(\frac{1}{|\vect x-\vect x'|}\right)=\frac{\vect x-\vect x'}{|\vect x-\vect x'|^3}$$
$$\nabla^2 = \frac 1{r^2}\pder r\left(r^2\pder r\right)+\frac{1}{r^2\sin\theta}\pder\theta\left(\sin\theta\pder\theta\right)+\frac{1}{r^2\sin\theta}\frac{\partial^2}{\partial\phi^2};\quad\nabla^2\left(\frac{1}{|\vect x-\vect x'|}\right)=-4\pi\delta(\vect x-\vect x')$$
$$\nabla^2=\frac 1\rho\pder \rho\left(\rho\pder\rho\right)+\frac{1}{\rho^2}\frac{\partial^2}{\partial \phi^2}+\frac{\partial^2}{\partial z^2};\quad R(\rho) = AJ_\nu(k\rho)+BN_\nu(k\rho);\quad Z(z)=e^{\pm kz};\quad Q(\phi)=e^{\pm i\nu\phi}$$
$$\Phi(\vect x) = k\int_V\rho(\vect x')G(\vect x,\vect x')\,d^3x'+\frac{1}{4\pi}\oint_{\partial V}\left[G(\vect x,\vect x')\pder[\Phi]{n'}-\Phi(\vect x')\frac{\partial G(\vect x,\vect x')}{\partial n'} \right]da';\quad G_D(\vect x,\vect x')|_{x'\in\partial V}=0$$
$$\Phi = \frac{U(r)}{r}P(\theta)Q(\phi);\quad Q=e^{\pm im\phi};\quad U = Ar^{l+1}+Br^{-l};\quad P(\theta)=P_l^m(\cos\theta)$$
$$\Phi(r,\theta) = \sum_{l=0}^\infty{[A_lr^l+B_lr^{-(l+1)}]P_l(\cos\theta)};\quad A_l=\frac{2l+1}{2}\int_0^\pi\Phi(r,\theta)|_{BC}P_l(\cos\theta)$$
$$Y_{lm}(\theta,\phi)=\sqrt{\frac{2l+1}{4\pi}\frac{(l-m)!}{(l+m)!}}P_l^m(\cos\theta)e^{im\phi};\quad Y_{l-m} = (-1)^mY*_{lm}$$
$$\frac{1}{|\vect x-\vect x'|}=4\pi\sum_{l=0}^\infty\sum_{m=-l}^l\frac{1}{2l+1}\frac{r^l_<}{r^{l+1}_>}Y^*_{lm}(\theta',\phi')Y_{lm}(\theta,\phi)$$
$$q'=-q\frac{R}{r_0};\quad r_0' = \frac{R^2}{r_0};\quad\sigma=-\frac{q}{4\pi R^2}\frac{R}{r_0}\frac{1-R^2/r_0^2}{(1+R^2/r_0^2-2R/r_0\cos\gamma)^{3/2}}$$
$$P_l(x)=\frac{1}{2^ll!}\frac{d^l}{dx^l}(x^2-1)^l;\quad P_l^m(x)=(-1)^m(1-x^2)^{m/2}\frac{d^m}{dx^m}P_l(x);$$
$$\Phi(\vect x) = -k\int_{\partial V}D(\vect x')\,d\Omega;\quad \Delta\Phi = \frac{D}{\epo};\quad\vect p=\vect nD\,da'$$
$$\delta(r)=\begin{cases}\frac{1}{\frac{4\pi}{3}\gamma^3}&\quad r\le \gamma\\0&\quad r>\gamma\end{cases};\quad\frac{1}{|\vect x+\vect a|}=\frac{1}{x}+\vect a\cdot\nabla\left(\frac 1x\right)+...$$
\end{document}